\documentclass{article}
\usepackage[left=3cm,right=3cm,top=2cm,bottom=2cm]{geometry} % page settings
\usepackage{amsmath} % provides many mathematical environments & tools
\usepackage{graphicx}
\usepackage{mathrsfs}
\usepackage{amssymb}
\usepackage{algorithm}
\usepackage[noend]{algpseudocode}
\usepackage{mathtools}
\usepackage{textcomp}

\setlength{\parindent}{0mm}
\makeatletter
\setlength{\@fptop}{0pt}
\makeatother
\def\BState{\State\hskip-\ALG@thistlm}

\newcommand{\RNum}[1]{\uppercase\expandafter{\romannumeral #1\relax}}
\DeclarePairedDelimiter\ceil{\lceil}{\rceil}
\DeclarePairedDelimiter\floor{\lfloor}{\rfloor}


\begin{document}

\title{CSE 250A: Assignment 5}
\author{Jiaxu Zhu~~A53094655}
\date{\today}
\maketitle
%%%%%%%%%%%%%%%%%%%%%%%%%%%%%%%%%%%%%%%%%%%%%%%%%%%%%%%%%%%%%%%%%%%%%%%%%%%%%%%%%%%%%%%%%%%
\subsection*{5.1 EM algorithm}
\subparagraph*{(a)~Posterior probability}
\begin{eqnarray*}
	P(a,c|b,d) &=& \frac{P(a,c,b,d)}{P(b,d)}\\
	&=&\frac{P(a,c,b,d)}{\sum_{a',c'}P(a',b,c',d)}\\
	&=&\frac{P(a)P(b|a)P(c|a,b)P(d|b,c)}{\sum_{a',c'}P(a')P(b|a')P(c'|a',b)P(d|b,c')}
\end{eqnarray*}

\subparagraph*{(b)~Posterior probability}
\begin{eqnarray*}
	P(a|b,d) &=& \sum_{c'}P(a,c'|b,d)\\
	P(c|b,d) &=& \sum_{a'}P(a',c|b,d)\\ 
\end{eqnarray*}

\subparagraph*{(c)~Log-likelihood}
\begin{eqnarray*}
	\mathcal{L} &=& \sum_{t}\log P(B = b_t, D = d_t)\\
	&=& \sum_{t}\log \sum_{a', c'}P(A = a', B = b_t, C = c', D = d_t)\\
	&=& \sum_{t}\log \sum_{a',c'}P(A=a')P(B=b_t|A=a')P(C=c'|A=a',B=b_t)P(D=d_t|B=b_t,C=c')
\end{eqnarray*}

\subparagraph*{(d)~EM algorithm}
\subparagraph*{E-step}
\begin{eqnarray*}
	P(b,a|b_t, d_t) &=& I(b, b_t)P(a|b_t, d_t)\\
	P(c, a, b | b_t, d_t) &=& I(b, b_t)P(a, c|b_t, d_t)\\
	P(d, b, c | b_t, d_t) &=& I(b, b_t)I(d, d_t)P(c|b_t, d_t)\\
\end{eqnarray*}
\subparagraph*{M-step}
\begin{eqnarray*}
	P(b | a) &=& \frac{\sum_{t}P(b, a|b_t, d_t)}{\sum_{t}P(a|b_t, d_t)}\\
	&=& \frac{\sum_{t}I(b, b_t)P(a|b_t, d_t)}{\sum_{t}P(a|b_t, d_t)}\\
	P(c, a, b | b_t, d_t) &=& \frac{\sum_{t}P(c, b, a|b_t, d_t)}{\sum_{t}P(a, b|b_t, d_t)}\\
	&=& \frac{\sum_{t}I(b, b_t)P(a, c|b_t, d_t)}{\sum_{t}I(b, b_t)P(a|b_t, d_t)}\\
	P(d, b, c | b_t, d_t) &=& \frac{\sum_{t}P(d, c, b|b_t, d_t)}{\sum_{t}P(b, c|b_t, d_t)}\\
	&=& \frac{\sum_{t}I(b, b_t)I(d, d_t)P(c|b_t, d_t)}{\sum_{t}I(b, b_t)P(c|b_t, d_t)}\\
\end{eqnarray*}

\subsection*{5.2 EM algorithm for noisy-OR}
\subparagraph*{(a)}
\begin{eqnarray*}
	P(Y = 1| X) &=& \sum_{Z \in \{0,1\}^n}P(Y =1 ,Z | X)\\	
	&=& \sum_{Z \in \{0,1\}^n}P(Y =1 |Z , X) P(Z|X)\\
	&=& \sum_{Z \in \{0,1\}^n}P(Y=1|Z)P(Z|X)~~(d-separation~~\RNum{1})\\
	&=& \sum_{Z \in \{0,1\}^n}P(Y=1|Z)\prod_{i=1}^{n}P(Z_i|X_i)~~(d-separation~~\RNum{3})\\
	&=& 1- \sum_{Z \in \{0,1\}^n}P(Y=0|Z)\prod_{i=1}^{n}P(Z_i|X_i)~~(d-separation~~\RNum{3})\\
	&=& 1- P(Y=0|Z=\vec{0})\prod_{i=1}^{n}P(Z_i=0|X_i)\\
	&=& 1 - \prod_{i=1}^{n}(1-p_i)^{X_i}
\end{eqnarray*}

\subparagraph*{(b)}
\begin{eqnarray*}
	P(Z_i = 1, X_i = 1| X=x, Y=y) &=& P(x_i = 1)P(Z_i = 1|X=x, Y=y)\\
	&=& x_i \frac{P(Y=y|X=x, Z_i = 1)P(Z_i = 1|X=x)}{P(Y=y|X=x)}\\
\end{eqnarray*}

\subparagraph*{(c)}
\begin{eqnarray*}
	p_i &=& \frac{\sum_{t}P(Z_i=1, X_i=1| X=x^{(t)}, Y=y^{(t)})}{\sum_{t}P(X_i=1| X=x^{(t)}, Y=y^{(t)})}\\
	&=& \frac{\sum_{t}P(Z_i=1, X_i=1| X=x^{(t)}, Y=y^{(t)})}{\sum_{t}P(X_i=1)}\\
	&=& \frac{1}{T_i}\sum_{t}P(Z_i=1, X_i=1| X=x^{(t)}, Y=y^{(t)})
\end{eqnarray*}
where $T_i$ is the number of examples in which $X_i=1$.

\subparagraph*{(d)}
The completed version of table is shown in Tab. 1\ref{hw5.2}.
\begin{table}
	\centering
	\begin{tabular}{|p{1.2cm}|p{1.2cm}|p{1.2cm}|p{1.2cm}|p{1.2cm}|p{1.2cm}|p{1.2cm}|p{1.2cm}|p{1.2cm}|p{1.2cm}|}
		\hline
		\#  & 0 & 1 & 2 & 4 & 8 & 16 & 32 & 64\\
		\hline 
		 $\mathcal{L}$& -2.5709 & -0.6938 & -0.5442 & -0.5385 & -0.5372 & -0.5365 & -0.5363 & -0.5365\\
		\hline
	\end{tabular}
	\label{hw5.2}
	\caption{the log-likelihood}
\end{table}

\subsection*{5.3 EM algorithm for noisy-OR}
\subparagraph*{(a)}
\begin{eqnarray*}
	\cosh x &=& \frac{e^x + e^{-x}}{2}\\
	f(x) &=& \log \frac{e^x + e^{-x}}{2}\\
	f'(x) &=& \frac{2}{e^x + e^{-x}} \frac{e^x - e^{-x}}{2}\\
	&=& \frac{e^{2x}-1}{e^{2x}+1}\\
	f''(x) &=& \frac{2e^{2x}(e^{2x}+1) - 2e^{2x}(e^{2x}-1)}{(e^{2x}+1)^2}\\
	&=& \frac{4e^{2x}}{(e^{2x}+1)^2}
\end{eqnarray*}
Let $f'(x)=0$, we get $x=0$. And since $f''(x) \ge 0$, we can tell that minimum occurs at $x=0$.

\subparagraph*{(b)}
\begin{eqnarray*}
	f''(x) &=& \frac{4e^{2x}}{(e^{2x}+1)^2}\\
	&=& \left(\frac{2e^x}{e^{2x}+1}\right)^2\\
	&=& \left(\frac{1}{coshx}\right)^2\\
	&\le& 1
\end{eqnarray*}

\subparagraph*{(c)}

\end{document}

